\section{Proof of Hoeffdingâ€™s Inequality}
\begin{definition}
(Hoeffding's Inequality)
Let $X_{1},...,X_{m}$ be iid random variables such that $a_{i}<X<b_{i}$ with probability $1$. Let $S_{n} = \Sigma_{i=1}^{n}X_{i}$, then for any $t>0$,  
\begin{equation*}
    P(|S_{n} - E[S_{n}]|\geq t) \leq 2e^{- \frac{2t^2}{\Sigma_{i=1}^{n}(b_{i}-a_{i}^{2})}}
\end{equation*}
\end{definition}

\begin{proof}
The key to of this proof is the following upper bound: if $X$ is a random variable with $E[X]=0$ and $a \leq X \leq b,$ then
$$
E\left[e^{s X}\right] \leq e^{\frac{s^{2}(b-a)^{2}}{8}}
$$
To derive the upper bound, by the convexity of the exponential function,
$$
e^{s x} \leq \frac{x-a}{b-a} e^{s b}+\frac{b-x}{b-a} e^{s a}, \text { for } a \leq x \leq b
$$

Therefore,
$$
\begin{aligned}
E\left[e^{s X}\right] & \leq E\left[\frac{X-a}{b-a}\right] e^{s b}+E\left[\frac{b-X}{b-a}\right] e^{s a} \\
&=\frac{b}{b-a} e^{s a}-\frac{a}{b-a} e^{s b}, \text { since } E[X]=0 \\
&=\left(1-\theta+\theta e^{s(b-a)}\right) e^{-\theta s(b-a)}, \text { where } \theta=\frac{-a}{b-a}
\end{aligned}
$$
Now let
$$
u=s(b-a) \text { and define } \phi(u) \equiv-\theta u+\log \left(1-\theta+\theta e^{u}\right)
$$
Then we have
$$
E\left[e^{s X}\right] \leq\left(1-\theta+\theta e^{s(b-a)}\right) e^{-\theta s(b-a)}=e^{\phi(u)}
$$
Using Taylor's expansion:
$$
\phi(u)=\phi(0)+u \phi^{\prime}(0)+\frac{u^{2}}{2} \phi^{\prime \prime}(v) \text { for some } v \in[0, u]
$$

$$
\begin{aligned}
\phi^{\prime}(u) &=-\theta+\frac{\theta e^{u}}{1-\theta+\theta e^{u}} \Rightarrow \phi^{\prime}(u)=0 \\
\phi^{\prime \prime}(u) &=\frac{\theta e^{u}}{1-\theta+\theta e^{u}}\left(1-\frac{\theta e^{u}}{1-\theta+\theta e^{u}}\right) \\
&=\rho(1-\rho)
\end{aligned}
$$
$\mathrm{Now}, \phi^{\prime \prime}(u)$ is maximized by
$$
\rho=\frac{\theta e^{u}}{1-\theta+\theta e^{u}}=\frac{1}{2} \Rightarrow \phi^{\prime \prime}(u) \leq \frac{1}{4}
$$
So,
$$
\begin{aligned}
\phi(u) & \leq \frac{u^{2}}{8}=\frac{s^{2}(b-a)^{2}}{8} \\
\Rightarrow E\left[e^{s X}\right] & \leq e^{\frac{s^{2}(b-a)^{2}}{8}}
\end{aligned}
$$

Now, we can apply this upper bound to derive Hoeffding's inequality.
$$
\begin{aligned}
P\left(S_{n}-E\left[S_{n}\right] \geq t\right) & \leq e^{-s t} \prod_{i=1}^{n} E\left[e^{s\left(L_{i}-E\left[L_{i}\right]\right)}\right] \\
& \leq e^{-s t} \prod_{i=1}^{n} e^{\frac{s^{2}\left(b_{i}-a_{i}\right)^{2}}{8}} \\
&=e^{-s t} e^{s^{2} \sum_{i=1}^{n} \frac{\left(b_{i}-a_{i}\right)^{2}}{8}} \\
&=e^{\frac{-2 t^{2}}{\sum_{i=1}^{n}\left(b_{i}-a_{i}\right)^{2}}} \\
& \text { by choosing } s=\frac{4 t}{\sum_{i=1}^{n}\left(b_{i}-a_{i}\right)^{2}}
\end{aligned}
$$
Similarly, $P\left(E\left[S_{n}\right]-S_{n} \geq t\right) \leq e^{\frac{-2 t^{2}}{\sum_{i=1}^{n}\left(b_{i}-a_{i}\right)^{2}}}$ . This completes the proof of the Hoeffding's theorem. 
\end{proof}